<?xml version="1.0" encoding="UTF-8"?>

<!DOCTYPE rdf:RDF [
  <!ENTITY vol "http://sweet.jpl.nasa.gov/2.0/geolVolcano.owl">  
  <!ENTITY top "http://sweet.jpl.nasa.gov/2.0/top.owl">  
  <!ENTITY sys "http://sweet.jpl.nasa.gov/2.0/sciSystem.owl">  
  <!ENTITY sysd "http://sweet.jpl.nasa.gov/2.0/sciSystemDynamics.owl">  
  <!ENTITY phys "http://sweet.jpl.nasa.gov/2.0/phys.owl">  
  <!ENTITY dur "http://sweet.jpl.nasa.gov/2.0/timeExtent.owl">  
  <!ENTITY ign "http://sweet.jpl.nasa.gov/2.0/geolPetrologyIgneous.owl">  
  <!ENTITY geol "http://sweet.jpl.nasa.gov/2.0/geol.owl">  
  <!ENTITY chem "http://sweet.jpl.nasa.gov/2.0/chem.owl">  
  <!ENTITY math "http://sweet.jpl.nasa.gov/2.0/math.owl">  
  <!ENTITY trans "http://sweet.jpl.nasa.gov/2.0/physTransport.owl">
  <!ENTITY etrans "http://sweet.jpl.nasa.gov/2.0/envirTransport.owl">
  <!ENTITY fail "http://sweet.jpl.nasa.gov/2.0/physSolidFailure.owl">
  <!ENTITY thermo "http://sweet.jpl.nasa.gov/2.0/physThermo.owl">
  <!ENTITY planet "http://sweet.jpl.nasa.gov/2.0/astroPlanet.owl">
  <!ENTITY owl "http://www.w3.org/2002/07/owl#">
  <!ENTITY rdf "http://www.w3.org/1999/02/22-rdf-syntax-ns#">
  <!ENTITY rdfs "http://www.w3.org/2000/01/rdf-schema#">
  <!ENTITY xsd "http://www.w3.org/2001/XMLSchema#">
]>

<rdf:RDF xml:base="&vol;"
         xmlns:top="&top;"
         xmlns:sys="&sys;"
         xmlns:sysd="&sysd;"
         xmlns:owl="&owl;"
         xmlns:rdf="&rdf;"
         xmlns:rdfs="&rdfs;"
         xmlns:xsd="&xsd;"
	 xmlns:fail="&fail;"
	 xmlns:trans="&trans;"
	 xmlns:etrans="&etrans;"
         xmlns:phys="&phys;"
         xmlns:dur="&dur;"
         xmlns:ign="&ign;"
         xmlns:math="&math;"
         xmlns:chem="&chem;"
         xmlns:geol="&geol;"
         xmlns:thermo="&thermo;"
         xmlns:planet="&planet;"
         xmlns:vol="&vol;"
>
<!-- Ontology Information -->
  <owl:Ontology rdf:about=""
                owl:versionInfo="2.0">
     <owl:imports rdf:resource="&thermo;"/>
     <owl:imports rdf:resource="&planet;"/>
     <owl:imports rdf:resource="&phys;"/>
     <owl:imports rdf:resource="&dur;"/>
     <owl:imports rdf:resource="&math;"/>
     <owl:imports rdf:resource="&geol;"/>
     <owl:imports rdf:resource="&chem;"/>
     <owl:imports rdf:resource="&ign;"/>
     <owl:imports rdf:resource="&top;"/>
     <owl:imports rdf:resource="&sys;"/>
     <owl:imports rdf:resource="&sysd;"/>
     <owl:imports rdf:resource="&fail;"/>
     <owl:imports rdf:resource="&trans;"/>
     <owl:imports rdf:resource="&etrans;"/>
  </owl:Ontology>

<!-- Phenomena -->
  <owl:Class rdf:ID="Dormant">
    <rdfs:subClassOf rdf:resource="&sys;#ActivityLevel"/>
  </owl:Class>

  <owl:Class rdf:ID="Eruption">
    <rdfs:subClassOf rdf:resource="#VolcanicActivity"/>
    <rdfs:subClassOf>
      <owl:Restriction>
        <owl:someValuesFrom rdf:resource="&trans;#MassFlux"/>
        <owl:onProperty rdf:resource="&trans;#hasFlux"/>
      </owl:Restriction>
    </rdfs:subClassOf>
    <rdfs:subClassOf>
      <owl:Restriction>
        <owl:someValuesFrom rdf:resource="&thermo;#ThermalFlux"/>
        <owl:onProperty rdf:resource="&trans;#hasFlux"/>
      </owl:Restriction>
    </rdfs:subClassOf>
    <owl:equivalentClass rdf:resource="#VolcanicEruption"/>
    <rdfs:comment xml:lang="en">Moderate to violent ejection of solid or very viscous hot fragments of new lava in short-lived, cannon-like bursts. Ash and fine ash are emitted with gases and ascend to form a cauliflower-like eruption cloud.</rdfs:comment>
  </owl:Class>
  <owl:Class rdf:ID="VolcanicEruption"/>

  <owl:Class rdf:ID="Extinct">
    <rdfs:subClassOf rdf:resource="&sys;#ActivityLevel"/>
    <rdfs:comment xml:lang="en">[Volcanic Activity] - Type 3 - Extinct volcanoes are those that scientists consider unlikely to erupt again, because the volcano no longer has a lava supply. [Wikipedia]</rdfs:comment>
  </owl:Class>

  <owl:Class rdf:ID="FlankEruption">
    <rdfs:subClassOf rdf:resource="#Eruption"/>
    <rdfs:comment xml:lang="en">An eruption from the side of a volcano (in contrast to a summit eruption.)</rdfs:comment>
  </owl:Class>

  <owl:Class rdf:ID="Geothermal">
    <rdfs:subClassOf rdf:resource="&thermo;#Heat"/>
    <rdfs:comment xml:lang="en">In geology, geothermal refers to heat sources within the planet. Strictly speaking, geo-thermal necessarily refers to the Earth but the concept may be applied to other planets. Geothermal is technically an adjective (e.g., geothermal energy) but in U.S. English the word has attained frequent use as a noun (otherwise expressed as g. heat, g. source, or geotherm). The planet's internal heat was originally generated during its accretion, due to gravitational binding energy, and since then additional heat has continued to be generated by the radioactive decay of elements such as uranium, thorium, and potassium. The heat flow from the interior to the surface is only 1/20,000 as great as the energy received from the Sun.</rdfs:comment>
  </owl:Class>

  <owl:Class rdf:ID="GeothermalPhenomena">
    <rdfs:subClassOf rdf:resource="&geol;#GeospherePhenomena"/>
    <rdfs:subClassOf>
      <owl:Restriction>
        <owl:onProperty rdf:resource="&phys;#hasPhysicalProcess" />
        <owl:allValuesFrom rdf:resource="#GeothermalProcess" />
      </owl:Restriction>
    </rdfs:subClassOf>
    <rdfs:comment xml:lang="en">Geothermal phemomena is an instance where the geothermal process is observed including volanoes, geysers and gas plumes. [Wikipedia]</rdfs:comment>
  </owl:Class>

  <owl:Class rdf:ID="GeothermalProcess">
    <rdfs:subClassOf rdf:resource="&thermo;#ThermalProcess"/>
    <rdfs:subClassOf rdf:resource="&geol;#GeologicProcess"/>
    <rdfs:comment xml:lang="en">A geological process whereby heat flows constantly from its sources within the Earth to the surface. [Wikipedia]</rdfs:comment>
  </owl:Class>

  <owl:Class rdf:ID="Hotspot">
    <rdfs:subClassOf rdf:resource="#VolcanicPlume"/>
    <rdfs:subClassOf>
      <owl:Restriction>
        <owl:allValuesFrom rdf:resource="#LinearVolcanicChain"/>
        <owl:onProperty rdf:resource="&planet;#hasPlanetaryRealm"/>
      </owl:Restriction>
    </rdfs:subClassOf>
    <rdfs:subClassOf>
      <owl:Restriction>
        <owl:allValuesFrom rdf:resource="&ign;#AnorogenicIgneousRock"/>
        <owl:onProperty rdf:resource="&chem;#hasSubstance"/>
      </owl:Restriction>
    </rdfs:subClassOf>
    <rdfs:comment xml:lang="en">In geology, a hotspot is a location on the Earth's surface that has experienced active volcanism for a long period of time. [Wikipedia]</rdfs:comment>
  </owl:Class>

  <owl:Class rdf:ID="LavaOfTephra">
    <rdfs:subClassOf rdf:resource="&trans;#MassFlux"/>
    <rdfs:subClassOf rdf:resource="&ign;#Lava"/>
    <rdfs:comment xml:lang="en">Tephra is air-fall material (of any size) produced by a volcanic eruption regardless of composition or fragment size. [Wikipedia]</rdfs:comment>
  </owl:Class>

  <owl:Class rdf:about="#MantlePlume">
    <rdfs:subClassOf rdf:resource="#VolcanicPlume"/>
    <owl:equivalentClass rdf:resource="#MantleThermalPlume"/>
    <rdfs:subClassOf>
      <owl:Restriction>
        <owl:onProperty rdf:resource="&planet;#hasPlanetaryRealm" />
        <owl:allValuesFrom rdf:resource="&geol;#Mantle" />
      </owl:Restriction>
    </rdfs:subClassOf>
    <rdfs:comment xml:lang="en">A mantle plume is an upwelling of abnormally hot rock within the Earth's mantle. As the heads of mantle plumes can partly melt when they reach shallow depths, they are thought to be the cause of volcanic centers known as hotspots and probably also to have caused flood basalts. [Wikipedia]</rdfs:comment>
  </owl:Class>
  <owl:Class rdf:about="#MantleThermalPlume"/>

  <owl:Class rdf:ID="MagmaMotion">
    <rdfs:subClassOf rdf:resource="#VolcanicActivity"/>
  </owl:Class>

  <owl:Class rdf:ID="Magmatic">
    <rdfs:subClassOf rdf:resource="#Eruption"/>
    <rdfs:comment xml:lang="en">Eruption Type 1 - produce juvenile clasts during explosive decompression from gas release. [Wikipedia]</rdfs:comment>
  </owl:Class>

  <owl:Class rdf:ID="NueeArdenteEruption"/>
  <owl:Class rdf:ID="PeleeanEruption">
    <rdfs:subClassOf rdf:resource="#Eruption"/>
    <owl:equivalentClass rdf:resource="#NueeArdenteEruption"/>
    <rdfs:comment xml:lang="en">In a Peléan eruption or nuée ardente (glowing cloud) eruptions a large amount of gas, dust, ash, and lava fragments are blown out of a central crater, fall back, and form avalanches that move downslope at speeds as great as 160 km per hour. These eruptions are usually associated with silicic magmas. A name for some pyroclastic flows is nuée ardente (French for "glowing cloud"); this was first used to describe the disastrous 1902 eruption of Mount Pelée on Martinique.[3] These pyroclastic flows glowed red in the dark. [Wikipedia]</rdfs:comment>
  </owl:Class>

  <owl:Class rdf:ID="PhreaticEruption">
    <rdfs:comment xml:lang="en">Phreatic eruption is an explosion that follows the transformation of groundwater into steam. No incandescent or juvenile material is erupted.</rdfs:comment>
    <rdfs:subClassOf rdf:resource="#Eruption"/>
  </owl:Class>

  <owl:Class rdf:ID="SteamBlastEruption">
    <owl:equivalentClass rdf:resource="#PhreaticEruption"/>
    <rdfs:comment xml:lang="en">A series of hundreds of steam explosions preceding an eruption of the volcano A less intense geothermal event may result in a mud volcano. In 1949, Thomas Jaggar described this kind of activity as steam-blast eruptions. [Wikipedia]</rdfs:comment>
  </owl:Class>

  <owl:Class rdf:ID="PhreatomagmaticEruption">
    <rdfs:subClassOf rdf:resource="#Eruption"/>
    <rdfs:comment xml:lang="en">Eruption Type 2 - Ejection of entrained particles during steam eruptions. [Wikipedia]</rdfs:comment>
  </owl:Class>


  <owl:Class rdf:ID="PlinianEruption">
    <rdfs:comment xml:lang="en">Plinian eruptions are characterized by paroxysmal ejection of large volume of ash and pumice as a well-defined eruption column or "jet;" often precedes caldera collapse. The resulting tephra fallout covers an area of more than 500 square kilometers.</rdfs:comment>
    <rdfs:subClassOf rdf:resource="#Eruption"/>
  </owl:Class>

  <owl:Class rdf:ID="Repose">
    <rdfs:subClassOf rdf:resource="&dur;#Duration"/>
    <rdfs:comment xml:lang="en">The interval of time between volcanic eruptions.</rdfs:comment>
  </owl:Class>

  <owl:Class rdf:ID="StrombolianEruption">
    <rdfs:subClassOf rdf:resource="#Eruption"/>
    <rdfs:comment xml:lang="en">Strombolian Eruptions are characterised by huge clots of molten lava bursting from the summit crater to form luminous arcs through the sky. Collecting on the flanks of the cone, lava clots combine to stream down the slopes in molten rivulets. The explosions are driven by bursts of gas slugs that rise faster than surrounding magma</rdfs:comment>
  </owl:Class>

  <owl:Class rdf:ID="SummitEruption">
    <rdfs:subClassOf rdf:resource="#Eruption"/>
  </owl:Class>

  <owl:Class rdf:ID="Surge">
    <rdfs:subClassOf rdf:resource="#VolcanicPlume"/>
    <rdfs:comment xml:lang="en">A ring-shaped cloud of gas and suspended solid debris that moves radially outward at high velocity as a density flow from the base of a vertical eruption column accompanying a volcanic eruption or crater formation.</rdfs:comment>
  </owl:Class>

  <owl:Class rdf:ID="Vent">
    <rdfs:subClassOf rdf:resource="&fail;#Crack"/>
  </owl:Class>

  <owl:Class rdf:ID="VolcanicActivity">
    <rdfs:subClassOf rdf:resource="#Volcanism"/>
    <rdfs:comment xml:lang="en">A popular way of classifying magmatic volcanoes is by their frequency of eruption or Volcanic Activity. [Wikipedia]</rdfs:comment>
  </owl:Class>

  <owl:Class rdf:about="#VolcanicChain">
    <rdfs:subClassOf rdf:resource="&geol;#GeologicProvince"/>
    <owl:equivalentClass rdf:resource="#VolcanicArc"/>
    <rdfs:comment xml:lang="en">Island arcs that develop along the edges of a continent (for example, large parts of the Andes/ Central American/ Canadian mountain chain) may be known as a volcanic arc or volcanic chain. [Wikipedia]</rdfs:comment>
  </owl:Class>
  <owl:Class rdf:ID="VolcanicArc"/>

  <owl:Class rdf:about="#VolcanicField">
    <rdfs:subClassOf rdf:resource="&geol;#GeologicProvince"/>
    <rdfs:comment xml:lang="en">A volcanic field is a spot of the earth's crust that is prone to localized volcanic activity. They usually contain 10 to 100 volcanoes, such as cinder cones and are usually in clusters. Lava flows may also occur. They may occur as a monogenetic volcanic field or a polygenetic volcanic field. [Wikipedia]</rdfs:comment>
  </owl:Class>

  <owl:Class rdf:ID="VolcanicPhenomena">
    <rdfs:subClassOf rdf:resource="&geol;#GeospherePhenomena"/>
    <rdfs:subClassOf>
      <owl:Restriction>
        <owl:onProperty rdf:resource="&geol;#hasGeologicProcess"/>
        <owl:allValuesFrom rdf:resource="#Volcanism" />
      </owl:Restriction>
    </rdfs:subClassOf>
    <rdfs:comment xml:lang="en">A geophysical phenomena involving the extrusion of rock that tends to form mountains or features like mountains over a period of time. [Wikipedia]</rdfs:comment>
  </owl:Class>

  <owl:Class rdf:ID="Volcanism">
    <rdfs:subClassOf rdf:resource="&geol;#GeologicProcess"/>
    <owl:equivalentClass rdf:resource="#Vulcanism"/>
  </owl:Class>
  <owl:Class rdf:ID="Vulcanism"/>

  <owl:Class rdf:ID="VolcanicPlume">
    <rdfs:subClassOf rdf:resource="#VolcanicActivity"/>
    <rdfs:comment xml:lang="en">An eruption column of hot volcanic ash and gas emitted into the atmosphere during an explosive volcanic eruption. [Wikipedia]</rdfs:comment>
    <rdfs:subClassOf rdf:resource="&etrans;#Plume"/>
  </owl:Class>

  <owl:ObjectProperty rdf:ID="hasVolcanicActivity">
    <rdfs:subPropertyOf rdf:resource="&geol;#hasGeologicalPhenomena"/>
  </owl:ObjectProperty>

<!-- Realm -->
  <owl:Class rdf:ID="CentralVolcano">
    <rdfs:subClassOf rdf:resource="#Volcano"/>
    <rdfs:comment xml:lang="en">A volcano constructed by the ejection of debris and lava flows from a central point, forming a more or less symmetrical volcano.</rdfs:comment>
  </owl:Class>

  <owl:Class rdf:ID="CompoundVolcano">
    <rdfs:subClassOf rdf:resource="#Volcano"/>
    <rdfs:comment xml:lang="en">A volcano that consists of a complex of two or more vents, or a volcano that has an associated volcanic dome, either in its crater or on its flanks.</rdfs:comment>
  </owl:Class>

  <owl:Class rdf:ID="Monogenetic">
    <rdfs:subClassOf rdf:resource="#Volcano"/>
    <rdfs:comment xml:lang="en">A volcano built by a single eruption.</rdfs:comment>
  </owl:Class>

  <owl:Class rdf:ID="Stratovolcano">
    <rdfs:subClassOf rdf:resource="#Volcano"/>
    <rdfs:comment xml:lang="en">A volcano composed of both lava flows and pyroclastic material.</rdfs:comment>
  </owl:Class>

  <owl:Class rdf:ID="VolcanicSystem">
    <rdfs:subClassOf rdf:resource="&geol;#GeologicFeature"/>
    <rdfs:subClassOf>
      <owl:Restriction>
        <owl:allValuesFrom rdf:resource="#Eruption"/>
        <owl:onProperty rdf:resource="&top;#hasPhenomena"/>
      </owl:Restriction>
    </rdfs:subClassOf>
  </owl:Class>

  <owl:Class rdf:ID="Volcano">
    <rdfs:subClassOf rdf:resource="#VolcanicField"/>
    <rdfs:subClassOf>
      <owl:Restriction>
        <owl:onProperty rdf:resource="&chem;#hasPrimarySubstance"/>
        <owl:someValuesFrom rdf:resource="&ign;#Magma"/>
      </owl:Restriction>
    </rdfs:subClassOf>
    <rdfs:comment xml:lang="en">A volcano is an opening, or rupture, in a planet's surface or crust, which allows hot, molten rock, ash, and gases to escape from below the surface. Volcanic activity involving the extrusion of rock tends to form mountains or features like mountains over a period of time. [Wikipedia]</rdfs:comment>
  </owl:Class>

  <owl:Class rdf:about="#SubaqueousVolcano">
    <rdfs:subClassOf rdf:resource="#Volcano"/>
  </owl:Class>

  <owl:Class rdf:about="#Caldera">
    <rdfs:subClassOf rdf:resource="&geol;#GeologicFeature"/>
  </owl:Class>

  <owl:Class rdf:about="#LinearVolcanicChain">
    <rdfs:subClassOf rdf:resource="#VolcanicChain"/>
    <rdfs:comment xml:lang="en">Where this association of flood basalts with continental rifting is observed, it is not uncommon to find linear chains of volcanic islands  [Wikipedia]</rdfs:comment>
  </owl:Class>

<!-- Substance -->
  <owl:Class rdf:about="#VolcanicDeposit">
    <rdfs:subClassOf rdf:resource="&sysd;#Deposit"/>
    <rdfs:comment xml:lang="en">Volcanic deposits are molten rock (lava), solid rocks and ash which surround a volcano crater. [Wikipedia]</rdfs:comment>
  </owl:Class>

  <owl:Class rdf:about="#Ashfall">
    <rdfs:subClassOf rdf:resource="#Ejecta"/>
    <rdfs:comment xml:lang="en">Volcanic ash that has fallen through the air from an eruption cloud. A deposit so formed is usually well sorted and layered.</rdfs:comment>
  </owl:Class>

  <owl:Class rdf:about="#AshFlow">
    <rdfs:subClassOf rdf:resource="#DebrisFlow"/>
    <rdfs:comment xml:lang="en">A turbulent mixture of gas and rock fragments, most of which are ash-sized particles, ejected violently from a crater or fissure. The mass of pyroclastics is normally of very high temperature and moves rapidly down the slopes or even along a level surface.</rdfs:comment>
  </owl:Class>

  <owl:Class rdf:about="#Block">
    <rdfs:subClassOf rdf:resource="#Ejecta"/>
    <rdfs:comment xml:lang="en">Angular chunk of solid rock ejected during an eruption.</rdfs:comment>
  </owl:Class>

  <owl:Class rdf:about="#Bomb">
    <rdfs:subClassOf rdf:resource="#Ejecta"/>
    <rdfs:comment xml:lang="en">Fragment of molten or semi-molten rock, 2 1/2 inches to many feet in diameter, which is blown out during an eruption. Because of their plastic condition, bombs are often modified in shape during their flight or upon impact.</rdfs:comment>
  </owl:Class>

  <owl:Class rdf:about="#DebrisAvalanche">
    <rdfs:subClassOf rdf:resource="#DebrisFlow"/>
    <rdfs:comment xml:lang="en">A rapid and unusually sudden sliding or flowage of unsorted masses of rock and other material. As applied to the major avalanche involved in the eruption of Mount St. Helens, a rapid mass movement that included fragmented cold and hot volcanic rock, water, snow, glacier ice, trees, and some hot pyroclastic material. Most of the May 18, 1980 deposits in the upper valley of the North Fork Toutle River and in the vicinity of Spirit Lake are from the debris avalanche.</rdfs:comment>
  </owl:Class>

  <owl:Class rdf:about="#DebrisFlow">
    <rdfs:subClassOf rdf:resource="&trans;#MassFlux"/>
    <rdfs:comment xml:lang="en">A mixture of water-saturated rock debris that flows downslope under the force of gravity (also called lahar or mudflow).</rdfs:comment>
  </owl:Class>

  <owl:Class rdf:about="#Ejecta">
    <rdfs:subClassOf rdf:resource="&chem;#Mixture"/>
    <rdfs:subClassOf>
      <owl:Restriction>
        <owl:onProperty rdf:resource="&top;#hasPhenomena" />
        <owl:allValuesFrom rdf:resource="#VolcanicActivity" />
      </owl:Restriction>
    </rdfs:subClassOf>
    <rdfs:comment xml:lang="en">In volcanology, particles that came out of a volcanic vent, traveled through the air or under water, and fell back on the ground surface or on the ocean floor. [Wikipedia]</rdfs:comment>
  </owl:Class>

  <owl:Class rdf:about="#EruptionCloud">
    <rdfs:subClassOf rdf:resource="#Ejecta"/>
    <rdfs:comment xml:lang="en">The column of gases, ash, and larger rock fragments rising from a crater or other vent. If it is of sufficient volume and velocity, this gaseous column may reach many miles into the stratosphere, where high winds will carry it long distances.</rdfs:comment>
  </owl:Class>

  <owl:Class rdf:about="#Hypoclastite">
    <rdfs:subClassOf rdf:resource="#VolcanicDeposit"/>
    <rdfs:comment xml:lang="en">A deposit formed by the flowing or intrusion of lava or magma into water, ice, or water-saturated sediment and its consequent granulation or shattering into small angular fragments.</rdfs:comment>
  </owl:Class>

  <owl:Class rdf:about="#Lahar">
    <rdfs:subClassOf rdf:resource="#Mudflow"/>
    <rdfs:comment xml:lang="en">A torrential flow of water-saturated volcanic debris down the slope of a volcano in response to gravity. A type of mudflow.</rdfs:comment>
  </owl:Class>

  <owl:Class rdf:about="#Mudflow">
    <rdfs:subClassOf rdf:resource="#DebrisFlow"/>
    <rdfs:comment xml:lang="en">A flowage of water-saturated earth material possessing a high degree of fluidity during movement. A less-saturated flowing mass is often called a debris flow. A mudflow originating on the flank of a volcano is properly called a lahar.</rdfs:comment>
  </owl:Class>

</rdf:RDF>
